theories/TraceEquiv.v
@@ -18,248 +18,59 @@ Section TraceEquiv.
   Definition step_equiv G P :=
     forall a, (exists G', step a G G') <-> (exists P', lstep a P P').
 
+  Lemma g_stequiv G E Q :
+    proj_cfg G == Some (E, Q) ->
+    step_equiv G (E, Q).
+  Proof.
+    rewrite /step_equiv/proj_cfg.
+    case G_E: (proj_env G) => [E'|//].
+    case G_Q: (queue_contents G [fmap]%fmap) => [Q'|//].
+    move=>/eqP=>[[EE' QQ']].
+    move: EE' QQ' G_E G_Q=>->->/eqP-H1/eqP-H2 a; split.
+    (* Testing *)
+    move=>[G']. elim=>//.
+    About step_ind1.
+    (* End Testing *)
+    - move=>[G' H]; move: G H H1 H2; elim/gty_ind1=>//.
+      + by move=> St; case Eq: (g_end (option lbl)) _ / St =>//.
+      + by move=> v St; case Eq: (g_var (option lbl) v) _ / St =>//.
+      + move=> G Ih.
+        admit.
+      + move=> lb p q Ks Ih.
+        admit.
+        (*
+        move=> lb p q Ks t Gp Cont Proj Queue.
+        move: (proj_send Proj) => [KsL] /andP-[Ks_KsL E_KsL].
+        move: (lookup_prjall Cont Ks_KsL) => [Lp /andP-[Gp_Lp KsL_Lp]].
+        move: (doact_send E_KsL KsL_Lp) => [E'' E_send].
+        by exists (E'', enq Q (p, q) (lb, t)); constructor.
+         *)
+    - admit.
+  Admitted.
+
+  Inductive Roll : renv -> renv -> Prop :=
+  | RR : forall p P Q,
+
   Definition trace_equiv G P : Prop :=
     forall tr, g_lts tr G <-> l_lts tr P.
 
-  Fixpoint add_head p (Q : MsgQ) :=
-    match Q with
-    | [::] => [:: (p.1, [:: p.2])]
-    | h :: t => if h.1 == p.1 then (h.1, p.2 :: h.2) :: t
-                else h :: add_head p t
-    end.
-
-  Notation msg m := (m.1, inr m.2).
-  Notation lab m l := (m.1, inl l).
-
-  Fixpoint merge_mq (Q : MsgQ) (Qs : seq (option MsgQ)) :=
-    match Qs with
-    | [::] => Some Q
-    | h :: t => if h == Some Q then merge_mq Q t
-                else None
-    end.
-
-  Definition merge_q (Q : seq (option MsgQ)) :=
-    match Q with
-    | [::] => Some [::]
-    | h :: t =>
-      match h with
-      | Some q => merge_mq q t
-      | None => None
-      end
-    end.
-
-  Fail Fixpoint msg_proj G (p : role) : option MsgQ :=
-    match G with
-    | rg_end
-    | rg_var _ => Some [::]
-    | rg_msg _ G
-    | rg_rec G => msg_proj G p
-    | rg_rcv m G =>
-      if m.snd == p
-      then match msg_proj G p with
-           | Some Q => Some (add_head (msg m) Q)
-           | None => None
-           end
-      else msg_proj G p
-    | rg_brn m K =>
-      merge_q [seq msg_proj lG.2 p | lG <- K]
-    | rg_alt lb m K =>
-      if m.snd == p
-      then match merge_q [seq msg_proj lG.2 p | lG <- K] with
-           | Some Q => Some (add_head (lab m lb) Q)
-           | None => None
-           end
-      else merge_q [seq msg_proj lG.2 p | lG <- K]
-    end.
-
-  Fail Definition project_rcv p r L :=
-    let: (p1, q, t) := p in
-    if p1 == q
-    then None
-    else if q == r
-         then ml_recv p1 t L
-         else L.
-
-  Fail Definition project_alt (p : g_prefix) (r : role) (K : seq (lbl * option l_ty)) :=
-    let: ((p, q), t) := p in
-    if p == q
-    then None
-    else if q == r
-         then ml_brn p K
-         else merge_all K.
-
-  Notation lbv v := (l_var (bv _ 0)).
-
-  Fail Fixpoint rg_proj G (r : role) : option l_ty :=
-    match G with
-    | rg_end => Some l_end
-    | rg_var v => Some (l_var v)
-    | rg_rec G => let: L := rg_proj G r in
-                  if L == Some (lbv 0) then None else ml_rec L
-    | rg_rcv m G => project_rcv m r (rg_proj G r)
-    | rg_msg m G => project_msg m r (rg_proj G r)
-    | rg_brn p K => let: KL := [seq (X.1, rg_proj X.2 r) | X <- K]
-                    in project_brn p r KL
-    | rg_alt lb p K => let: KL := [seq (X.1, rg_proj X.2 r) | X <- K]
-                       in project_alt p r KL
-    end.
-
-  Fail Definition q_proj G r :=
-    match msg_proj G r, rg_proj G r with
-    | Some Q, Some L => Some (Q, L)
-    | _, _ => None
-    end.
-
-
-  Fail Inductive mq_proj p : rg_ty -> MsgQ -> l_ty -> Prop :=
-  | prj_end :
-      mq_proj p rg_end [::] l_end
-  | prj_var  v :
-      mq_proj p (rg_var v) [::] (l_var v)
-  | prj_rec G Q L :
-      L != lbv 0 ->
-      mq_proj p G Q L ->
-      mq_proj p (rg_rec G) Q (l_rec L)
-  | prj_msg1 q x G Q L :
-      p != q ->
-      mq_proj p G Q L ->
-      mq_proj p (rg_msg ((p, q), x) G) Q (l_send q x L)
-  | prj_msg2 q x G Q L :
-      p != q ->
-      mq_proj p G Q L ->
-      mq_proj p (rg_msg ((q, p), x) G) Q (l_recv q x L)
-  | prj_msg3 f t x G Q L :
-      f != t ->
-      f != p ->
-      f != p ->
-      mq_proj p G Q L ->
-      mq_proj p (rg_msg ((f, t), x) G) Q L
-  | prj_rcv1 q x G Q L :
-      p != q ->
-      mq_proj p G Q L ->
-      mq_proj p (rg_rcv ((p, q), x) G) (add_head ((p, q), inr x) Q) L
-  | prj_rcv2 q x G Q L :
-      p != q ->
-      mq_proj p G Q L ->
-      mq_proj p (rg_rcv ((q, p), x) G) Q (l_recv q x L)
-  | prj_rcv3 f t x G Q L :
-      f != t ->
-      f != p ->
-      f != p ->
-      mq_proj p G Q L ->
-      mq_proj p (rg_rcv ((f, t), x) G) Q L
-  | prj_brn1 q x KG Q KL :
-      p != q ->
-      proj_alts p KG Q KL ->
-      mq_proj p (rg_brn ((p, q), x) KG) Q (l_sel q KL)
-  | prj_brn2 q x KG Q KL :
-      p != q ->
-      proj_alts p KG Q KL ->
-      mq_proj p (rg_brn ((q, p), x) KG) Q (l_brn q KL)
-  | prj_brn3 f t x KG Q L :
-      f != t ->
-      f != p ->
-      p != t ->
-      proj_all p KG Q L ->
-      mq_proj p (rg_brn ((f, t), x) KG) Q L
-  | prj_alt1 l q x KG Q KL L :
-      p != q ->
-      lookup l KL == Some L ->
-      proj_alts p KG Q KL ->
-      mq_proj p (rg_alt l ((p, q), x) KG) (add_head ((p, q), inl l) Q) L
-  | prj_alt2 l q x KG Q KL :
-      p != q ->
-      proj_alts p KG Q KL ->
-      mq_proj p (rg_alt l ((q, p), x) KG) Q (l_brn q KL)
-  | prj_alt3 l f t x KG Q L :
-      f != t ->
-      f != p ->
-      p != t ->
-      proj_all p KG Q L ->
-      mq_proj p (rg_alt l ((f, t), x) KG) Q L
-  with
-  proj_alts p : seq (lbl * rg_ty) -> MsgQ -> seq (lbl * l_ty) -> Prop :=
-  | prj_nil G Q L l :
-      mq_proj p G Q L ->
-      proj_alts p [:: (l, G)] Q [:: (l, L)]
-  | prj_cons KG Q KL l G L :
-      mq_proj p G Q L ->
-      proj_alts p KG Q KL ->
-      proj_alts p ((l, G) :: KG) Q ((l, L) :: KL)
-  with
-  proj_all p : seq (lbl * rg_ty) -> MsgQ -> l_ty -> Prop :=
-  | prj_all_nil G Q L l :
-      mq_proj p G Q L ->
-      proj_all p [:: (l, G)] Q L
-  | prj_all_cons KG Q l G L :
-      mq_proj p G Q L ->
-      proj_all p KG Q L ->
-      proj_all p ((l, G) :: KG) Q L.
-
-  Fail Derive Inversion mqproj_inv with (forall p G Q L, mq_proj p G Q L) Sort Prop.
-  Fail Derive Inversion mqproj_end_inv with (forall p Q L, mq_proj p rg_end Q L) Sort Prop.
-  Fail Derive Inversion mqproj_var_inv with (forall v p Q L, mq_proj p (rg_var v) Q L) Sort Prop.
-  Fail Derive Inversion mqproj_rec_inv with (forall p G Q L, mq_proj p (rg_rec G) Q L) Sort Prop.
-  Fail Derive Inversion projalts_inv with (forall p K Q L, proj_alts p K Q L) Sort Prop.
-  Fail Derive Inversion projall_inv with (forall p K Q L, proj_all p K Q L) Sort Prop.
-
-  Fail Lemma qproj_equiv p G Q L : q_proj G p == Some (Q, L) <-> mq_proj p G Q L.
   (*
-  Proof.
-    suff : (msg_proj G p == Some Q) && (rg_proj G p == Some L)
-           <-> mq_proj p G Q L.
-    {
-      suff : (msg_proj G p == Some Q) && (rg_proj G p == Some L)
-             <-> q_proj G p == Some (Q, L)
-        by move=>->.
-      rewrite /q_proj; split; case: (msg_proj G p); case: (rg_proj G p)=>//Q'.
-      by rewrite andbC.
-    }
-    move: G Q L; elim/rgty_ind2 =>///=.
-    - move=> Q L; rewrite /q_proj/=; split.
-      + by move=>/andP-[/eqP-[<-] /eqP-[<-]]; constructor.
-      + by elim/mqproj_end_inv.
-    - move=> v Q L; rewrite /q_proj/=; split.
-      + by move=>/andP-[/eqP-[<-] /eqP-[<-]]; constructor.
-      + by elim/mqproj_var_inv; rewrite !eq_refl.
-    - move=> G Ih Q L; split.
-      + move=>/andP-[GQ]; case: ifP=>// neqL; rewrite /ml_rec => H.
-        have [L' GL']: exists L', rg_proj G p == Some L'
-            by move: H; case: (rg_proj G p) => // L' _; exists L'.
-        move: GQ GL' H neqL (Ih Q L') =>/eqP-> /eqP-> /eqP-[<-] {Ih}.
-        rewrite -[Some _ == Some _]/(L' == _) (rwP negPf) !eq_refl => L'lvar.
-        by move=>[/(_ is_true_true)-Ih _]; constructor.
-      + elim/mqproj_rec_inv=>_ G0 Q0 L0 Neq /Ih/andP-[->/eqP->] _ _ _{G0 Q0 L}/=.
-        by rewrite -[Some _ == _]/(L0 == _) (negPf Neq).
-  Admitted.
    *)
+  Lemma g_trequiv G : forall P, proj_cfg G == Some P -> trace_equiv G P.
+  Proof.
+    move=>[E Q]; rewrite /trace_equiv/proj_cfg.
+    case G_E: (proj_env G) => [E'|//].
+    case G_Q: (queue_contents G [fmap]%fmap) => [Q'|//].
+    move=>/eqP=>[[EE' QQ']].
+    move: EE' QQ' G_E G_Q=>->->/eqP-H1/eqP-H2 tr; split.
 
-  Fail Inductive Proj G : seq role -> MsgQ * PEnv -> Prop :=
-  | proj_end : Proj G [::] ([::], [::])
-  | proj_next p ps Q1 Q2 L P :
-      mq_proj p G Q1 L -> Proj G ps (Q2, P) ->
-      Proj G (p :: ps) (Q1 ++ Q2, insert (p, L) P).
+    cofix Ch.
+    + move=> trcG; move: trcG H1 H2 Ch; case.
+      * rewrite /proj_env/= =>/eqP-[<-] /eqP-[<-] _; constructor.
+      * move=> a t G0 G' step trc.
+      * move=>/=. _.
 
-  Fail Definition Projection G P := (forall x, x \in rg_parts G <-> x \in unzip1 P.2)
-                               /\ Proj G (unzip1 P.2) P.
 
-  Definition q_union (Q1 Q2 : MsgQ) := Q1 ++ Q2.
-
-  Fail Fixpoint q_project G ps :=
-    match ps with
-    | [::] => Some ([::], [::])
-    | h :: t => match q_proj G h , q_project G t with
-                | Some (Q', L), Some (Q, P) => Some (q_union Q Q', insert (h, L) P)
-                | _, _ => None
-                end
-    end.
-
-  Fail Fixpoint is_valid G :=
-    match G with
-    | rg_var _ => false
-    | rg_rec G => is_valid G && (G != rg_end)
-    | _ => true
-    end.
 
   Fail Definition q_projection G :=
     if is_valid G then q_project G (rg_parts G)
